LibDecomp.v
@@ -1,9 +1,4 @@
-(** ** Specific redefinition of usual tactics. *)
-
-(** Note that for example !!induction h doesn not work because
-    "destruct" is not a ltac function by itself, it is already a
-    notation. Hence the special definitions below for this kind of
-    tactics: induction ddestruct inversion etc. *)
+(** ** A specific variant of decompose. Which only decomposes logical connectives. does *)
 
 Ltac decomp_logicals h :=
   match type of h with
@@ -25,20 +20,11 @@ Ltac decomp_logicals h :=
   | _ => idtac
   end.
 
-(* decompose and ex and or at once. TODO: generalize. *)
-(* clear may fail if h is not a hypname *)
-(* Tactic Notation "decomp" hyp(h) :=
-   (!! (idtac;decomp_logicals h)). *) (* Why do I need this idtac? Without it no rename happens. *)
-
-Ltac decompose_clear c :=
-  let h := fresh "h_decomp" in
-  pose proof c as h;
-  decomp_logicals c; try clear h.
 (*
 Lemma foo : forall x, { aa:nat | (aa = x /\ x=aa) & (aa = aa /\ aa= x) } -> False.
 Proof.
-  intros x H. 
-  decomp H.
+  intros x h. 
+  pose proof h as h'.
 Abort.
 
 Lemma foo : { aa:False & True  } -> False.
